Corretness proof sepref

theories/Compositional_Structures/Basic_Modules/Elect_Module_Ref.thy
@@ -4,21 +4,43 @@ theory Elect_Module_Ref
 
 begin
 
+ \<comment> \<open>The elect module should not return just the reference to all alternatives
+  but a deep copy\<close>
 fun elect_module_ref :: "'a Electoral_Module_Ref" where
-  "elect_module_ref A p = RETURN (A, {}, {})"
+  "elect_module_ref A p =
+   FOREACH A
+     (\<lambda> x (e,r,d). RETURN ((insert x e), r, d)) ({},{},{})"
 
 lemma elect_module_ref_correct:
-  shows "(elect_module_ref, (\<lambda> A p. RETURN (elect_module A p)))
+  shows "(elect_module_ref, (\<lambda> A p. SPEC (\<lambda> res. res= elect_module A p)))
       \<in> elec_mod_relb"
   unfolding elect_module_ref.simps elect_module.simps
-  apply refine_vcg
-  by auto
+  apply (intro fun_relI)
+proof (rename_tac A' A pl pr)
+  fix A' A:: "'a set"
+  fix pl pr 
+  assume arel: "(A', A) \<in> \<langle>Id\<rangle>alt_set_rel"
+  from arel have aeq: "A' = A" by (auto simp add: alt_set_rel_def in_br_conv)
+  from arel have fina: "finite A" by (auto simp add: alt_set_rel_def in_br_conv)
+  have "(FOREACH A' (\<lambda>x (e, r, d). RETURN (insert x e, r, d)) ({}, {}, {}),
+        SPEC (\<lambda>res. res = (A, {}, {})))
+       \<in> \<langle>Id\<rangle>nres_rel"
+  apply (refine_vcg FOREACH_rule[where I = "\<lambda>it (e,r,d). e = A' - it \<and> r = {} \<and> d = {}"])
+    by (auto simp add: aeq fina)
+  from this show "(FOREACH A' (\<lambda>x (e, r, d). RETURN (insert x e, r, d)) ({}, {}, {}),
+        SPEC (\<lambda>res. res = (A, {}, {})))
+       \<in> \<langle>\<langle>Id\<rangle>set_rel \<times>\<^sub>r \<langle>Id\<rangle>set_rel \<times>\<^sub>r \<langle>Id\<rangle>set_rel\<rangle>nres_rel"
+    by simp
+qed
+  
 
-sepref_definition em_sep is 
-  "uncurry elect_module_ref" :: "(hs.assn nat_assn)\<^sup>d *\<^sub>a (list_assn (array_assn nat_assn))\<^sup>k
+sepref_definition elect_sepref is 
+  "uncurry elect_module_ref" :: "(hs.assn nat_assn)\<^sup>k *\<^sub>a (list_assn (array_assn nat_assn))\<^sup>k
     \<rightarrow>\<^sub>a ((hs.assn nat_assn) \<times>\<^sub>a (hs.assn nat_assn) \<times>\<^sub>a (hs.assn nat_assn))"
   unfolding elect_module_ref.simps
   apply (rewrite in "\<hole>" hs.fold_custom_empty)+
   by sepref
+
+lemmas elect_sepref_correct = elect_sepref.refine[FCOMP elect_module_ref_correct]
 
 end
